isabelle/Chapter13_4_Evaluation.thy
@@ -1,152 +1,6 @@
-theory Chapter13_3_Evaluation
-imports Chapter13_2_Typechecking
+theory Chapter13_4_Evaluation
+imports Chapter13_3_PatternMatching
 begin
-
-fun is_val :: "expr => bool"
-where "is_val (Var v) = False"
-    | "is_val Zero = True"
-    | "is_val (Succ n) = is_val n"
-    | "is_val (IsZ e0 e1 et) = False"
-    | "is_val (Lam t b) = True"
-    | "is_val (Ap e1 e2) = False"
-    | "is_val (Fix t b) = False"
-    | "is_val Triv = True"
-    | "is_val (Pair e1 e2) = (is_val e1 & is_val e2)"
-    | "is_val (ProjL e) = False"
-    | "is_val (ProjR e) = False"
-    | "is_val (Abort t e) = False"
-    | "is_val (InL t t' e) = is_val e"
-    | "is_val (InR t t' e) = is_val e"
-    | "is_val (Match e rs) = False"
-
-lemma canonical_nat: "typecheck env e Nat ==> is_val e ==> e = Zero | (EX v. typecheck env v Nat & is_val v & e = Succ v)"
-by (induction e, auto)
-
-lemma canonical_arr: "typecheck env e (Arr t1 t2) ==> is_val e ==> (EX v. e = Lam t1 v & typecheck (extend_at env 0 t1) v t2)"
-by (induction e, auto)
-
-lemma canonical_unit: "typecheck env e Unit ==> is_val e ==> e = Triv"
-by (induction e, auto)
-
-lemma canonical_prod: "typecheck env e (Prod t1 t2) ==> is_val e ==> (EX e1 e2. e = Pair e1 e2 & typecheck env e1 t1 & typecheck env e2 t2 & is_val e1 & is_val e2)"
-by (induction e, auto)
-
-lemma canonical_void: "typecheck env e Void ==> ~ is_val e"
-by (induction e, auto)
-
-lemma canonical_sum: "typecheck env e (Sum t1 t2) ==> is_val e ==> 
-      (EX e'. e = InL t1 t2 e' & is_val e' & typecheck env e' t1) | (EX e'. e = InR t1 t2 e' & is_val e' & typecheck env e' t2)"
-by (induction e, auto)
-
-inductive typecheck_subst :: "(nat, type) assoc => expr list => type list => bool"
-where tsubn [simp]: "typecheck_subst env [] []"
-    | tsubc [simp]: "typecheck env e t ==> typecheck_subst env es ts ==> typecheck_subst env (e # es) (t # ts)"
-
-inductive_cases [elim!]: "typecheck_subst e [] t"
-inductive_cases [elim!]: "typecheck_subst e (x # y) t"
-
-lemma [simp]: "typecheck_subst env e1 t1 ==> typecheck_subst env e2 t2 ==> typecheck_subst env (e1 @ e2) (t1 @ t2)"
-by (induction env e1 t1 rule: typecheck_subst.induct, simp_all)
-
-inductive matches :: "expr list => patn => expr => bool"
-where [simp]: "matches [] Wild e"
-    | [simp]: "matches [e] PVar e"
-    | [simp]: "matches [] PTriv Triv"
-    | [simp]: "matches s1 p1 e1 ==> matches s2 p2 e2 ==> matches (s1 @ s2) (PPair p1 p2) (Pair e1 e2)"
-    | [simp]: "matches s p e ==> matches s (PInL p) (InL t t' e)"
-    | [simp]: "matches s p e ==> matches s (PInR p) (InR t t' e)"
-
-inductive_cases [elim!]: "matches s Wild e"
-inductive_cases [elim!]: "matches s PVar e"
-inductive_cases [elim!]: "matches s PTriv e"
-inductive_cases [elim!]: "matches s (PPair x y) e"
-inductive_cases [elim!]: "matches s (PInL x) e"
-inductive_cases [elim!]: "matches s (PInR x) e"
-
-inductive no_match :: "expr => patn => bool"
-where [simp]: "no_match e1 p1 ==> no_match (Pair e1 e2) (PPair p1 p2)"
-    | [simp]: "no_match e2 p2 ==> no_match (Pair e1 e2) (PPair p1 p2)"
-    | [simp]: "no_match (InL t t' e) (PInR p)"
-    | [simp]: "no_match e p ==> no_match (InL t t' e) (PInL p)"
-    | [simp]: "no_match (InR t t' e) (PInL p)"
-    | [simp]: "no_match e p ==> no_match (InR t t' e) (PInR p)"
-
-lemma [simp]: "no_match (Pair e1 e2) (PPair p1 p2) ==> no_match e1 p1 | no_match e2 p2"
-by (auto, induction "Pair e1 e2" "PPair p1 p2" rule: no_match.induct, auto)
-
-lemma [simp]: "no_match (InL t t' e) (PInL p) = no_match e p"
-by (auto, induction "InL t t' e" "PInL p" rule: no_match.induct, simp)
-
-lemma [simp]: "no_match (InR t t' e) (PInR p) = no_match e p"
-by (auto, induction "InR t t' e" "PInR p" rule: no_match.induct, simp)
-
-lemma "types_from_pat p t ts ==> typecheck env e t ==> is_val e ==> (EX s. typecheck_subst env s ts & matches s p e) | no_match e p"
-proof (induction p t ts arbitrary: e rule: types_from_pat.induct)
-case tpwld
-  have "typecheck_subst env [] [] & matches [] Wild e" by simp
-  hence "EX s. typecheck_subst env s [] & matches s Wild e" by (rule exI)
-  thus ?case by simp
-next case (tpvar t)
-  hence "typecheck_subst env [e] [t] & matches [e] PVar e" by simp
-  hence "EX s. typecheck_subst env s [t] & matches s PVar e" by (rule exI)
-  thus ?case by simp
-next case tptrv
-  hence "e = Triv" by (simp add: canonical_unit)
-  hence "typecheck_subst env [] [] & matches [] PTriv e" by simp
-  hence "EX s. typecheck_subst env s [] \<and> matches s PTriv e" by (rule exI)
-  thus ?case by simp
-next case (tppar p1 t1 ts1 p2 t2 ts2)
-  hence "(EX e1 e2. e = Pair e1 e2 & typecheck env e1 t1 & typecheck env e2 t2 & is_val e1 & is_val e2)" by (simp add: canonical_prod)
-  with tppar show ?case
-  proof auto
-    fix e1 e2 s1 s2
-    assume "!!e. typecheck env e t1 ==> is_val e ==> (EX s. typecheck_subst env s ts1 & matches s p1 e) | no_match e p1"
-       and "typecheck env e1 t1"
-       and "is_val e1"
-    hence A: "(EX s. typecheck_subst env s ts1 & matches s p1 e1) | no_match e1 p1" by auto
-    assume "!!e. typecheck env e t2 ==> is_val e ==> (EX s. typecheck_subst env s ts2 & matches s p2 e) | no_match e p2"
-       and "typecheck env e2 t2"
-       and "is_val e2"
-    hence B: "(EX s. typecheck_subst env s ts2 & matches s p2 e2) | no_match e2 p2" by auto
-    assume C: "~ no_match (Pair e1 e2) (PPair p1 p2)"
-    from A C have "EX s. typecheck_subst env s ts1 & matches s p1 e1" by auto
-    moreover from B C have "EX s. typecheck_subst env s ts2 & matches s p2 e2" by auto
-    ultimately show "EX s. typecheck_subst env s (ts1 @ ts2) & matches s (PPair p1 p2) (Pair e1 e2)"
-    proof auto
-      fix s1 s2
-      assume "typecheck_subst env s1 ts1"
-         and "matches s1 p1 e1"
-         and "typecheck_subst env s2 ts2"
-         and "matches s2 p2 e2"
-      hence "typecheck_subst env (s1 @ s2) (ts1 @ ts2) & matches (s1 @ s2) (PPair p1 p2) (Pair e1 e2)" by simp
-      thus "EX s. typecheck_subst env s (ts1 @ ts2) & matches s (PPair p1 p2) (Pair e1 e2)" by auto
-    qed
-  qed
-next case (tpinl p t1 ts t2)
-  from tpinl have "(EX e'. e = InL t1 t2 e' & is_val e' & typecheck env e' t1) | (EX e'. e = InR t1 t2 e' & is_val e' & typecheck env e' t2)" by (simp add: canonical_sum)
-  with tpinl show ?case
-  proof (cases "EX e'. e = InL t1 t2 e'", auto)
-    fix e'
-    assume "!!e. typecheck env e t1 ==> is_val e ==> (EX s. typecheck_subst env s ts & matches s p e) | no_match e p"
-       and "~ no_match e' p"
-       and "is_val e'"
-       and "typecheck env e' t1"
-    hence "EX s. typecheck_subst env s ts & matches s p e'" by auto
-    thus "EX s. typecheck_subst env s ts & matches s (PInL p) (InL t1 t2 e')" by auto
-  qed
-next case (tpinr p t2 ts t1)
-  from tpinr have "(EX e'. e = InL t1 t2 e' & is_val e' & typecheck env e' t1) | (EX e'. e = InR t1 t2 e' & is_val e' & typecheck env e' t2)" by (simp add: canonical_sum)
-  with tpinr show ?case
-  proof (cases "EX e'. e = InR t1 t2 e'", auto)
-    fix e'
-    assume "!!e. typecheck env e t2 ==> is_val e ==> (EX s. typecheck_subst env s ts & matches s p e) | no_match e p"
-       and "~ no_match e' p"
-       and "is_val e'"
-       and "typecheck env e' t2"
-    hence "EX s. typecheck_subst env s ts & matches s p e'" by auto
-    thus "EX s. typecheck_subst env s ts & matches s (PInR p) (InR t1 t2 e')" by auto
-  qed
-qed
 
 inductive eval :: "expr => expr => bool"
 where esuc [simp]: "eval n n' ==> eval (Succ n) (Succ n')"
@@ -166,6 +20,9 @@ where esuc [simp]: "eval n n' ==> eval (Succ n) (Succ n')"
     | eabt [simp]: "eval e e' ==> eval (Abort t e) (Abort t e')"
     | einl [simp]: "eval e e' ==> eval (InL t t' e) (InL t t' e')"
     | einr [simp]: "eval e e' ==> eval (InR t t' e) (InR t t' e')"
+    | emt1 [simp]: "eval e e' ==> eval (Match e rs) (Match e' rs)"
+    | emt2 [simp]: "is_val e ==> matches s p e ==> eval (Match e (Rule p e2 # rs)) (apply_subst s e2)"
+    | emt3 [simp]: "is_val e ==> no_match e p ==> eval (Match e rs) e' ==> eval (Match e (Rule p e2 # rs)) e'"
 
 theorem preservation: "eval e e' ==> typecheck env e t ==> typecheck env e' t"
 proof (induction e e' arbitrary: t env rule: eval.induct)
@@ -207,6 +64,38 @@ next case eabt
 next case einl
   thus ?case by auto
 next case einr
+  thus ?case by auto
+next case (emt1 e e' rs)
+  hence "EX t1. typecheck env e t1 & typecheck_rules env rs t1 t" by auto
+  thus ?case
+  proof auto
+    fix t1
+    assume "typecheck env e t1"
+       and "typecheck_rules env rs t1 t"
+    moreover with emt1 have "typecheck env e' t1" by simp
+    ultimately show "typecheck env (Match e' rs) t" by simp
+  qed
+next case (emt2 e s p e2 rs)
+  hence "EX t1 ts. typecheck env e t1 & types_from_pat p t1 ts & typecheck (extend_env ts env) e2 t & typecheck_rules env rs t1 t" by auto
+  thus ?case
+  proof auto
+    fix t1 ts
+    assume "typecheck env e t1"
+       and "types_from_pat p t1 ts"
+       and A: "typecheck (extend_env ts env) e2 t"
+    hence "is_val e ==> (EX s. typecheck_subst env s ts & matches s p e) | no_match e p" by simp
+    with emt2 have "EX s. typecheck_subst env s ts & matches s p e" by simp
+    with A show "typecheck env (apply_subst s e2) t"
+    proof auto
+      fix sa
+      assume "typecheck_subst env sa ts" 
+         and "matches sa p e"
+         and "typecheck (extend_env ts env) e2 t"
+      (* s = sa ! *)
+      show "typecheck env (apply_subst s e2) t" by simp sorry
+    qed
+  qed
+next case emt3
   thus ?case by auto
 qed
 
